proofs/compiler/end_to_end.v
@@ -68,6 +68,7 @@ Require Import
   stack_alloc_proof_2
   compiler_proof
   it_compiler_proof
+  it_compiler_proof_2
 .
 Require allocation.
 
